compiler/backend/proofs/source_to_sourceProofsScript.sml
@@ -2,7 +2,8 @@
   Correctness proofs for floating-point optimizations
 *)
 
-open source_to_sourceIcingTheory fpOptTheory fpOptPropsTheory semanticPrimitivesTheory evaluateTheory
+open source_rewriterTheory source_to_sourceTheory fpOptTheory fpOptPropsTheory
+     fpSemPropsTheory semanticPrimitivesTheory evaluateTheory
      evaluatePropsTheory terminationTheory fpSemPropsTheory;
 open preamble;
 
@@ -35,12 +36,6 @@ Theorem isPureExpList_reverse[simp]:
 Proof
   Induct_on `es` \\ fs[isPureExp_def]
   \\ rpt gen_tac \\ EQ_TAC \\ simp[]
-QED
-
-Theorem triple_case_eq[local]:
-  (case a of |Rval c1 => (x,y,f c1) | Rerr c2 => (x,y,g c2)) = (x,y,case a of | Rval c1 => f c1 | Rerr c2 => g c2)
-Proof
-  Cases_on `a` \\ fs[]
 QED
 
 (**
@@ -90,33 +85,35 @@ end
 
 local
   val eval_goal =
-    ``\ (s1:'a state) env fps1 expl.
-        ! s2 fps2 r.
-          evaluate s1 env fps1 expl = (s2, fps2, r) ==>
+    ``\ (s1:'a semanticPrimitives$state) env expl.
+        ! s2 r.
+          evaluate s1 env expl = (s2, r) ==>
           isPureExpList expl /\
           r <> Rerr (Rabort Rtype_error) ==>
-          ! (s:'a state) (fps3:fp_state).
-            fps3.rws = fps1.rws /\
-            fps3.canOpt = fps1.canOpt /\
-            (! x. x <= (fps2.choices - fps1.choices) ==>
-              fps3.opts x = fps1.opts x) ==>
+          ! (s:'a semanticPrimitives$state).
+            s.fp_state.rws = s1.fp_state.rws /\
+            s.fp_state.canOpt = s1.fp_state.canOpt /\
+            (! x. x <= (s2.fp_state.choices - s1.fp_state.choices) ==>
+              s.fp_state.opts x = s1.fp_state.opts x) ==>
             ? fpOpts.
-              evaluate s env fps3 expl =
-                (s, fps2 with <| opts := fpOpts; choices := fps3.choices + (fps2.choices - fps1.choices) |>, r)``;
+              evaluate s env expl =
+                (s with <| fp_state := s.fp_state with
+                  <| opts := fpOpts; choices := s.fp_state.choices + (s2.fp_state.choices - s1.fp_state.choices)|> |>, r)``;
   val eval_match_goal =
-    ``\ (s1:'a state) env fps1 v pl err_v.
-        ! s2 fps2 r.
+    ``\ (s1:'a semanticPrimitives$state) env v pl err_v.
+        ! s2 r.
           isPurePatExpList pl /\
-          evaluate_match s1 env fps1 v pl err_v = (s2, fps2, r) ==>
+          evaluate_match s1 env v pl err_v = (s2, r) ==>
           r <> Rerr (Rabort Rtype_error) ==>
-          ! (s:'a state) (fps3:fp_state).
-            fps3.rws = fps1.rws /\
-            fps3.canOpt = fps1.canOpt /\
-            (! x. x <= (fps2.choices - fps1.choices) ==>
-              fps3.opts x = fps1.opts x) ==>
+          ! (s:'a semanticPrimitives$state).
+            s.fp_state.rws = s1.fp_state.rws /\
+            s.fp_state.canOpt = s1.fp_state.canOpt /\
+            (! x. x <= (s2.fp_state.choices - s1.fp_state.choices) ==>
+              s.fp_state.opts x = s1.fp_state.opts x) ==>
               ? fpOpts.
-              evaluate_match s env fps3 v pl err_v =
-                (s, fps2 with <| opts := fpOpts; choices := fps3.choices + (fps2.choices - fps1.choices) |>, r)``;
+              evaluate_match s env v pl err_v =
+                (s with <| fp_state := s.fp_state with
+                  <| opts := fpOpts; choices := s.fp_state.choices + (s2.fp_state.choices - s1.fp_state.choices)|> |>, r)``;
   val indThm = terminationTheory.evaluate_ind
     |> ISPEC eval_goal |> SPEC eval_match_goal
   val isPureExpList_single_thm =
@@ -132,14 +129,14 @@ local
   val trivial =
     rpt strip_tac \\ rveq \\ fs[]
     \\ res_tac
-    \\ first_x_assum (qspec_then `s` assume_tac)
-    \\ fs[fp_state_component_equality];
+    \\ qexists_tac `fpOpts'`
+    \\ fs[fpState_component_equality, state_component_equality];
 in
 Theorem isPureExpList_swap_ffi:
-  (! s1 env fps1 expl.
-    ^eval_goal s1 env fps1 expl) /\
-  (! s1 env fps1 v pl err_v.
-    ^eval_match_goal s1 env fps1 v pl err_v)
+  (! s1 env expl.
+    ^eval_goal s1 env expl) /\
+  (! s1 env v pl err_v.
+    ^eval_match_goal s1 env v pl err_v)
 Proof
   irule indThm \\ rpt gen_tac \\ rpt conj_tac
   \\ rpt gen_tac \\ rpt strip_tac \\ fs[]
@@ -147,10 +144,10 @@ Proof
   \\ rpt strip_tac
   \\ fs[isPureExpList_single_thm]
   \\ TRY (first_x_assum irule \\ fs[Once isPureExp_def] \\ NO_TAC)
-  \\ TRY (fs[fp_state_component_equality] \\ NO_TAC)
-  \\ TRY (qpat_x_assum `_ = (_, _, _)` mp_tac)
+  \\ TRY (fs[fpState_component_equality, state_component_equality] \\ NO_TAC)
+  \\ TRY (qpat_x_assum `_ = (_, _)` mp_tac)
   >- (
-    ntac 3 (reverse TOP_CASE_TAC \\ fs[]) >- trivial
+    ntac 2 (reverse TOP_CASE_TAC \\ fs[]) >- trivial
     \\ TOP_CASE_TAC \\ fs[]
     \\ rpt strip_tac
     \\ last_x_assum (qspec_then `s` resolve_simple)
@@ -160,66 +157,66 @@ Proof
     \\ rename [`do_if (HD r) e2 e3 = SOME eR`]
     \\ `isPureExp eR` by (imp_res_tac do_if_cases \\ fs[])
     \\ res_tac \\ fs[]
-    \\ qmatch_goalsub_abbrev_tac `evaluate _ env fpsNew [_]`
-    \\ first_x_assum (qspec_then `fpsNew` resolve_simple)
+    \\ qmatch_goalsub_abbrev_tac `evaluate s_fpNew env [_]`
+    \\ first_x_assum (qspec_then `s_fpNew` resolve_simple)
     \\ unabbrev_all_tac \\ fs[state_component_equality]
     \\ disch_then impl_subgoal_tac
     >- fp_inv_tac
     \\ imp_res_tac evaluate_fp_opts_inv
     \\ trivial)
   >- (
-    ntac 3 (reverse TOP_CASE_TAC \\ fs[]) >- trivial
-    \\ ntac 3 (TOP_CASE_TAC \\ fs[])
+    ntac 2 (reverse TOP_CASE_TAC \\ fs[]) >- trivial
+    \\ ntac 2 (TOP_CASE_TAC \\ fs[])
     \\ rpt strip_tac \\ rveq \\ fs[isPureExpList_Cons_thm]
-    \\ first_x_assum (qspecl_then [`s`, `fps3`] impl_subgoal_tac)
+    \\ first_x_assum (qspec_then `s` impl_subgoal_tac)
     \\ TRY (rpt conj_tac \\ fp_inv_tac \\ NO_TAC)
     \\ fs[]
     \\ rpt (first_x_assum (fn ithm => first_x_assum (fn thm => mp_then Any assume_tac thm ithm)))
-    \\ qmatch_goalsub_abbrev_tac `evaluate _ env fpsNew _`
-    \\ first_x_assum (qspecl_then [`s`, `fpsNew`] resolve_simple)
+    \\ qmatch_goalsub_abbrev_tac `evaluate s_fpNew env _`
+    \\ first_x_assum (qspecl_then [`s_fpNew`] resolve_simple)
     \\ unabbrev_all_tac
     \\ disch_then impl_subgoal_tac
     \\ TRY (rpt conj_tac \\ fp_inv_tac)
     \\ imp_res_tac evaluate_fp_opts_inv
-    \\ fs[fp_state_component_equality])
+    \\ fs[fpState_component_equality, state_component_equality])
   >- (
-    ntac 3 (reverse TOP_CASE_TAC \\ fs[]) >- trivial
+    ntac 2 (reverse TOP_CASE_TAC \\ fs[]) >- trivial
     \\ rpt strip_tac \\ rveq \\ fs[isPureExpList_Cons_thm]
-    \\ first_x_assum (qspecl_then [`s`, `fps3`] resolve_simple)
+    \\ first_x_assum (qspecl_then [`s`] resolve_simple)
     \\ disch_then impl_subgoal_tac
     >- (rpt conj_tac \\ fp_inv_tac)
     \\ fs[]
-    \\ qmatch_goalsub_abbrev_tac `evaluate_match _ env fpsNew _ _ _`
+    \\ qmatch_goalsub_abbrev_tac `evaluate_match s_fpNew env _ _ _`
     \\ first_x_assum impl_subgoal_tac >- fs[]
-    \\ first_x_assum (qspecl_then [`s`, `fpsNew`] resolve_simple)
+    \\ first_x_assum (qspecl_then [`s_fpNew`] resolve_simple)
     \\ unabbrev_all_tac
     \\ disch_then impl_subgoal_tac
     \\ TRY (rpt conj_tac \\ fp_inv_tac)
-    \\ fs[fp_state_component_equality]
+    \\ fs[fpState_component_equality, state_component_equality]
     \\ fp_inv_tac)
   >- (
-    ntac 3 (reverse TOP_CASE_TAC \\ fs[])
+    ntac 2 (reverse TOP_CASE_TAC \\ fs[])
     >- (rpt strip_tac \\ rveq \\ fs[]
         \\ first_x_assum drule
-        \\ disch_then (qspecl_then [`s`, `fps3 with canOpt := T`] assume_tac)
-        \\ fs[fp_state_component_equality]
-        \\ res_tac  \\ fs[fp_state_component_equality])
+        \\ disch_then (qspecl_then
+            [`s with fp_state := s.fp_state with canOpt := case annot of Opt => T | NoOpt => F`] impl_subgoal_tac)
+        >- (fs[fpState_component_equality])
+        \\ fs[fpState_component_equality, state_component_equality])
     \\ rpt strip_tac \\ rveq \\ fs[isPureExpList_Cons_thm]
     \\ res_tac
-    \\ last_x_assum (qspecl_then [`s`, `fps3 with canOpt := T`] assume_tac)
-    \\ fs[fp_state_component_equality]
-    \\ res_tac \\ fs[fp_state_component_equality])
-  >- (TOP_CASE_TAC \\ TRY trivial
-      \\ rpt strip_tac \\ rveq
-      \\ fs[fp_state_component_equality])
+    \\ last_x_assum (qspecl_then [`s with fp_state := s.fp_state with canOpt := case annot of Opt => T | NoOpt => F`] assume_tac)
+    \\ fs[fpState_component_equality]
+    \\ res_tac \\ fs[fpState_component_equality, state_component_equality])
+  >- (TOP_CASE_TAC \\ rpt strip_tac \\ rveq
+      \\ fs[fpState_component_equality, state_component_equality])
   >- (
-    ntac 3 (reverse TOP_CASE_TAC \\ fs[]) >- trivial
+    ntac 2 (reverse TOP_CASE_TAC \\ fs[]) >- trivial
     \\ ntac 2 (TOP_CASE_TAC \\ fs[])
     \\ rpt strip_tac \\ rveq \\ fs[]
     \\ first_x_assum drule
-    \\ disch_then (qspec_then `s` impl_subgoal_tac)
+    \\ impl_tac \\ fs[]
     \\ TRY (fp_inv_tac \\ NO_TAC)
-    \\ fs[fp_state_component_equality]
+    \\ disch_then assume_tac \\ fs[fpState_component_equality, state_component_equality]
     \\ rename [`do_log lop (HD v) e2 = SOME (Exp eR)`]
     \\ `eR = e2`
         by (qpat_x_assum `do_log _ _ _ = SOME (Exp eR)` mp_tac
@@ -227,54 +224,52 @@ Proof
             \\ rpt (TOP_CASE_TAC \\ fs[]))
     \\ rveq
     \\ first_x_assum drule \\ disch_then assume_tac
-    \\ qmatch_goalsub_abbrev_tac `evaluate _ env fpsNew _ = _`
-    \\ first_x_assum (qspecl_then [`s`, `fpsNew`] impl_subgoal_tac)
+    \\ qmatch_goalsub_abbrev_tac `evaluate s_fpNew env _ = _`
+    \\ first_x_assum (qspecl_then [`s_fpNew`] impl_subgoal_tac)
     \\ unabbrev_all_tac
     >- (fs[] \\ fp_inv_tac)
-    \\ fs[fp_state_component_equality]
+    \\ fs[fpState_component_equality, state_component_equality]
     \\ fp_inv_tac)
   >- (
-    ntac 3 (reverse TOP_CASE_TAC \\ fs[]) >- trivial
+    ntac 2 (reverse TOP_CASE_TAC \\ fs[]) >- trivial
     \\ TOP_CASE_TAC \\ fs[]
     >- (rveq \\ fs[isPureOp_def])
     \\ ntac 3 (reverse TOP_CASE_TAC \\ fs[])
     \\ imp_res_tac isPureOp_same_ffi
-    \\ first_x_assum (qspecl_then [`s`, `fps3`] assume_tac)
-    \\ rename [`evaluate st env fps (REVERSE es) = (s2, fps1, Rval _)`]
-    \\ TOP_CASE_TAC \\ Cases_on `fps1.canOpt` \\ fs[] \\ rpt strip_tac \\ rveq \\ fs[shift_fp_opts_def]
+    \\ first_x_assum (qspecl_then [`s`] assume_tac)
+    \\ rename [`evaluate st env (REVERSE es) = (s2, Rval _)`]
+    \\ TOP_CASE_TAC \\ Cases_on `s.fp_state.canOpt` \\ fs[] \\ rpt strip_tac \\ rveq \\ fs[shift_fp_opts_def]
     \\ first_x_assum impl_subgoal_tac
     \\ TRY (fp_inv_tac)
     \\ imp_res_tac evaluate_fp_opts_inv
-    \\ fs[shift_fp_opts_def, state_component_equality, fp_state_component_equality]
+    \\ fs[shift_fp_opts_def, state_component_equality, fpState_component_equality]
     \\ rpt (qpat_x_assum `! x. _ x = _ x` ( fn thm => fs[GSYM thm])))
   >- (
     TOP_CASE_TAC \\ fs[]
-    \\ ntac 3 (reverse TOP_CASE_TAC \\ fs[]) >- trivial
+    \\ ntac 2 (reverse TOP_CASE_TAC \\ fs[]) >- trivial
     \\ TOP_CASE_TAC \\ fs[]
     \\ rpt strip_tac \\ rveq
-    \\ first_x_assum drule \\ disch_then (qspec_then `s` impl_subgoal_tac)
+    \\ first_x_assum drule \\ disch_then impl_subgoal_tac
     >- fp_inv_tac
-    \\ fs[fp_state_component_equality])
+    \\ fs[fpState_component_equality, state_component_equality])
   >- (
-    ntac 3 (reverse TOP_CASE_TAC \\ fs[]) >- trivial
+    ntac 2 (reverse TOP_CASE_TAC \\ fs[]) >- trivial
     \\ rpt strip_tac \\ fs[]
-    \\ first_x_assum (qspecl_then [`s`, `fps3`] impl_subgoal_tac)
+    \\ first_x_assum (qspecl_then [`s`] impl_subgoal_tac)
     >- fp_inv_tac
     \\ fs[]
-    \\ qmatch_goalsub_abbrev_tac `evaluate _ _ fpsNew _ = _`
+    \\ qmatch_goalsub_abbrev_tac `evaluate s_fpNew _ _ = _`
     \\ first_x_assum impl_subgoal_tac \\ fs[]
-    \\ first_x_assum (qspecl_then [`s`, `fpsNew`] impl_subgoal_tac)
+    \\ first_x_assum (qspecl_then [`s_fpNew`] impl_subgoal_tac)
     \\ unabbrev_all_tac
     >- fp_inv_tac
-    \\ fs[fp_state_component_equality]
+    \\ fs[fpState_component_equality, state_component_equality]
     \\ fp_inv_tac)
   >- (
-    ntac 3 (TOP_CASE_TAC \\ fs[])
+    ntac 2 (TOP_CASE_TAC \\ fs[])
     \\ rpt strip_tac \\ fs[]
     \\ imp_res_tac (hd (CONJ_LIST 2 (EVAL_RULE isPurePat_ignores_ref)))
-    \\ fs[]
-    \\ res_tac \\ fs[fp_state_component_equality]
-    \\ fp_inv_tac)
+    \\ fs[])
 QED
 end
 
@@ -282,120 +277,125 @@ Theorem isPureExp_same_ffi:
   ! st1 st2 env fps1 fps2 e r.
     isPureExp e /\
     r <> Rerr (Rabort Rtype_error) /\
-    evaluate st1 env fps1 [e] = (st2, fps2, r) ==>
-    st1 = st2
+    evaluate st1 env [e] = (st2, r) ==>
+    st2 = st1 with fp_state := st2.fp_state
 Proof
   rpt strip_tac
   \\ first_assum (mp_then Any assume_tac (CONJUNCT1 (SIMP_RULE std_ss [] isPureExpList_swap_ffi)))
-  \\ first_x_assum (qspecl_then [`st1`, `fps1`] impl_subgoal_tac)
-  \\ fs[isPureExp_def] \\ fs[]
+  \\ first_x_assum (qspecl_then [`st1`] impl_subgoal_tac)
+  \\ fs[isPureExp_def] \\ fs[fpState_component_equality, state_component_equality]
 QED
 
 (**
   Next, we prove that it is always fine to append optimization by changing the
-  oracle.
+  oracle. We cannot use the same oracle as before.
+  This is because do_fprw accesses the rewrites from the state when executing
+  the schedule. If the previous schedule failed because the rewriter was not in
+  the list, the new execution must do the same to be semantics preserving.
+  Theorem do_fprw_append_opt in fpOptPropsTheory is critical for this proof.
 **)
 local
   val eval_goal =
-    ``\ (ffi:'a state) env fps el.
-        ! res ffi2 fps2 opt.
-          evaluate ffi env fps el = (ffi2, fps2, res) ==>
-          ? fpOptN fpOptN2.
-          evaluate ffi env (fps with <| rws := fps.rws ++ [opt]; opts := fpOptN |> ) el =
-            (ffi2, fps2 with <| rws := fps2.rws ++ [opt]; opts := fpOptN2 |>, res)``
+    ``\ (st1:'a state) env el.
+        ! res st2 opt.
+          evaluate st1 env el = (st2, res) ==>
+          ? fpOpt fpOpt2.
+          evaluate (st1 with fp_state := st1.fp_state with <| rws := st1.fp_state.rws ++ [opt]; opts := fpOpt |>) env el =
+            (st2 with fp_state := st2.fp_state with <| rws := st2.fp_state.rws ++ [opt]; opts := fpOpt2 |>, res)``
   val eval_match_goal =
-    ``\ (ffi:'a state) env fps v pl err_v.
-        ! res ffi2 fps2 opt.
-          evaluate_match ffi env fps v pl err_v = (ffi2, fps2, res) ==>
-          ? fpOptN fpOptN2.
-          evaluate_match ffi env (fps with <| rws := fps.rws ++ [opt]; opts := fpOptN |>) v pl err_v =
-            (ffi2, fps2 with <| rws := fps2.rws ++ [opt]; opts := fpOptN2 |>, res)``
+    ``\ (st1:'a state) env v pl err_v.
+        ! res st2 opt.
+          evaluate_match st1 env v pl err_v = (st2, res) ==>
+          ? fpOpt fpOpt2.
+          evaluate_match (st1 with fp_state := st1.fp_state with <| rws := st1.fp_state.rws ++ [opt]; opts := fpOpt |>) env v pl err_v =
+            (st2 with fp_state := st2.fp_state with <| rws := st2.fp_state.rws ++ [opt]; opts := fpOpt2|>, res)``
   val indThm = terminationTheory.evaluate_ind
     |> ISPEC eval_goal |> SPEC eval_match_goal
-  val eval_step =  ntac 3 (reverse TOP_CASE_TAC \\ fs[]);
+  val eval_step =  ntac 2 (reverse TOP_CASE_TAC \\ fs[]);
   val solve_simple =
     rpt strip_tac \\ rveq \\ fs[] \\ first_x_assum (qspec_then `opt` assume_tac) \\ fs[]
-    \\ qexists_tac `fpOptN` \\ qexists_tac `fpOptN2` \\ fs[];
+    \\ qexists_tac `fpOpt` \\ qexists_tac `fpOpt2` \\ fs[];
   val solve_complex =
-    rpt (qpat_x_assum `evaluate _ _ _ _ = _` kall_tac ORELSE
-            qpat_x_assum `evaluate_match _ _ _ _ _ _ = _` kall_tac)
+    rpt (qpat_x_assum `evaluate _ _ _ = _` kall_tac ORELSE
+            qpat_x_assum `evaluate_match _ _ _ _ _ = _` kall_tac)
     \\ rpt (last_x_assum (qspec_then `opt` assume_tac)) \\ fs[]
-    \\ (rename [`evaluate st1 env (fps1 with <| rws := _; opts := fpOpt1N |>) [e1] =
-                  (st2, fps2 with <| rws := _; opts := fps2opt |>, _)`,
-               `evaluate st2 _ (fps2 with <| rws := _; opts := fpOpt2N |>) _ =
-                  (st3, fps3 with <| rws := _; opts := fps3opt |>, _)`]
+    \\ (rename [`evaluate (st1 with fp_state := st1.fp_state with <| rws := _; opts := fpOpt1N |>) env [e1] =
+                  (st2 with fp_state := st2.fp_state with <| rws := _; opts := _ |>, _)`,
+                `evaluate (st2 with fp_state := st2.fp_state with <| rws := _; opts := fpOpt2N |>) _ _ =
+                  (st3 with fp_state := st3.fp_state with <| rws := _; opts := fpOpt3N |>, _)`]
         ORELSE
-      rename [`evaluate st1 env (fps1 with <| rws := _; opts := fpOpt1N |>) [e1] =
-                  (st2, fps2 with <| rws := _; opts := fps2opt |>, _)`,
-               `evaluate_match st2 env (fps2 with <| rws := _; opts := fpOpt2N |>) _ _ _=
-                  (st3, fps3 with <| rws := _; opts := fps3opt |>, _)`]
+      rename [`evaluate (st1 with fp_state := st1.fp_state with <| rws := _; opts := fpOpt1N |>) env [e1] =
+                  (st2 with fp_state := st2.fp_state with <| rws := _; opts := _ |>, _)`,
+               `evaluate_match (st2 with fp_state := st2.fp_state with <| rws := _; opts := fpOpt2N |>) env _ _ _=
+                  (st3 with fp_state := st3.fp_state with <| rws := _; opts := fpOpt3N |>, _)`]
       ORELSE
-      rename [`evaluate st1 env (fps1 with <| rws := _; opts := fpOpt1N |>) (REVERSE es) =
-                  (st2, fps2 with <| rws := _; opts := fps2opt |>, _)`,
-               `evaluate (dec_clock st2) _ (fps2 with <| rws := _; opts := fpOpt2N |>) _ =
-                  (st3, fps3 with <| rws := _; opts := fps3opt |>, _)`])
-    \\ qexists_tac `optUntil (fps2.choices - fps1.choices) fpOpt1N fpOpt2N`
-    \\ last_x_assum (mp_then Any assume_tac optUntil_evaluate_ok)
-    \\ first_x_assum (qspec_then `fpOpt2N` assume_tac)
-    \\ fs[fp_state_component_equality];
+      rename [`evaluate (st1 with fp_state := st1.fp_state with <| rws := _; opts := fpOpt1N |>) env (REVERSE es) =
+                  (st2 with fp_state := st2.fp_state with <| rws := _; opts := _ |>, _)`,
+               `evaluate (st2 with <| clock := st2.clock - 1; fp_state := st2.fp_state with <| rws := _; opts := fpOpt2N |> |>) _ _ =
+                  (st3 with fp_state := st3.fp_state with <| rws := _; opts := fpOpt3N|>, _)`])
+    \\ qexists_tac `optUntil (st2.fp_state.choices - st1.fp_state.choices) fpOpt1N fpOpt2N`
+    \\ rpt (first_x_assum (fn thm => (mp_then Any assume_tac optUntil_evaluate_ok thm) \\ mp_tac thm))
+    \\ rpt (first_x_assum (qspec_then `fpOpt2N` assume_tac))
+    \\ fs[fpState_component_equality, state_component_equality];
 in
 Theorem evaluate_fp_rws_append:
-  (! (ffi:'a state) env fps el.
-    ^eval_goal ffi env fps el) /\
-  (! (ffi:'a state) env fps v pl err_v.
-    ^eval_match_goal ffi env fps v pl err_v)
+  (! (ffi:'a state) env el.
+    ^eval_goal ffi env el) /\
+  (! (ffi:'a state) env v pl err_v.
+    ^eval_match_goal ffi env v pl err_v)
 Proof
   match_mp_tac indThm
-  \\ rpt strip_tac \\ fs[evaluate_def] \\ rpt strip_tac \\ rveq \\ fs[]
-  \\ TRY (qexists_tac `\ x. []` \\ fs[fp_state_component_equality] \\ NO_TAC)
-  \\ qpat_x_assum `_ = (_, _, _)` mp_tac
+  \\ rpt strip_tac \\ fs[evaluate_def] \\ rpt strip_tac \\ rveq \\ fs[fpState_component_equality]
+  \\ TRY (qexists_tac `\ x. []` \\ fs[fpState_component_equality, state_component_equality] \\ NO_TAC)
+  \\ qpat_x_assum `_ = (_, _)` mp_tac
   (* e1 :: e2 :: es *)
   >- (
     eval_step >- solve_simple
-    \\ ntac 2 (TOP_CASE_TAC) \\ fs[triple_case_eq] \\ rpt strip_tac \\ rveq
+    \\ ntac 2 (TOP_CASE_TAC)
+    \\ rpt strip_tac \\ rveq \\ fs[]
     \\ solve_complex)
   (* Raise e *)
   >- (eval_step \\ solve_simple)
   (* match *)
   >- (
-    ntac 3 (TOP_CASE_TAC \\ fs[]) >- solve_simple
+    ntac 2 (TOP_CASE_TAC \\ fs[]) >- solve_simple
     \\ reverse TOP_CASE_TAC \\ fs[] >- solve_simple
     \\ rpt strip_tac \\ fs[]
     \\ solve_complex)
   (* do_con_check *)
   >- (
       reverse TOP_CASE_TAC \\ fs[]
-      >- (rpt strip_tac \\ fs[fp_state_component_equality])
+      >- (rpt strip_tac \\ rveq \\ fs[fpState_component_equality, state_component_equality])
       \\ eval_step >- solve_simple
-      \\ TOP_CASE_TAC  \\ solve_simple)
+      \\ TOP_CASE_TAC \\ solve_simple)
   (* Variable lookup *)
-  >- (TOP_CASE_TAC \\ fs[fp_state_component_equality])
+  >- (TOP_CASE_TAC \\ fs[fpState_component_equality, state_component_equality])
   (* do_app *)
   >- (
     eval_step >- solve_simple
     \\ TOP_CASE_TAC \\ fs[]
     >- (TOP_CASE_TAC \\ fs[] >- solve_simple
         \\ ntac 2 (TOP_CASE_TAC \\ fs[]) >- solve_simple
-        \\ strip_tac \\ fs[]
+        \\ strip_tac \\ fs[dec_clock_def]
         \\ solve_complex)
     \\ TOP_CASE_TAC \\ fs[] >- solve_simple
     \\ ntac 3 (reverse TOP_CASE_TAC \\ fs[]) >- solve_simple
-    \\ qpat_x_assum `evaluate _ _ _ _ = _` kall_tac
+    \\ qpat_x_assum `evaluate _ _ _ = _` kall_tac
     \\ first_x_assum (qspec_then `opt` assume_tac) \\ fs[]
-    \\ rename [`evaluate st1 env (fps1 with <| rws := _; opts := fpOpt1N |>) (REVERSE es) =
-                  (st2, fps2 with <| rws := _; opts := fps2opt |>, _)`]
-    \\ Cases_on `fps2.canOpt` \\ fs[]
+    \\ rename [`evaluate (st1 with fp_state := st1.fp_state with <| rws := st1.fp_state.rws ++ [opt]; opts := fpOpt1 |>) env (REVERSE es) =
+                  (st2 with fp_state := _, _)`]
+    \\ Cases_on `st2.fp_state.canOpt` \\ fs[]
     >- (rpt strip_tac \\ rveq
-        \\ fs[shift_fp_opts_def, fp_state_component_equality]
+        \\ fs[shift_fp_opts_def, fpState_component_equality]
         \\ first_x_assum (mp_then Any assume_tac optUntil_evaluate_ok)
-        \\ Cases_on `do_fprw r (fps2.opts 0) fps2.rws`
+        \\ Cases_on `do_fprw r (st2.fp_state.opts 0) st2.fp_state.rws`
         \\ imp_res_tac do_fprw_append_opt
         \\ first_x_assum (qspec_then `[opt]` assume_tac) \\ fs[]
         \\ first_x_assum (qspec_then `\x. sched2` assume_tac)
-        \\ qexists_tac `optUntil (fps2.choices - fps1.choices) fpOpt1N (\x. sched2)`
-        \\ fs[fp_state_component_equality])
+        \\ qexists_tac `optUntil (st2.fp_state.choices - st1.fp_state.choices) fpOpt1 (\x. sched2)`
+        \\ fs[fpState_component_equality, state_component_equality])
     \\ rpt strip_tac \\ rveq
-    \\ qexists_tac `fpOpt1N` \\ fs[fp_state_component_equality])
+    \\ qexists_tac `fpOpt1` \\ fs[fpState_component_equality, state_component_equality])
   (* Log_op *)
   >- (
     eval_step >- solve_simple
@@ -421,15 +421,15 @@ Proof
     \\ solve_complex)
   (* ALL_DISTINCT *)
   >- (
-    reverse TOP_CASE_TAC >- fs[fp_state_component_equality]
+    reverse TOP_CASE_TAC >- fs[fpState_component_equality, state_component_equality]
     \\ strip_tac \\ fs[])
   >- (
     eval_step \\ strip_tac \\ rveq
-    \\ first_x_assum (qspec_then `opt'` assume_tac) \\ fs[]
-    \\ qexists_tac `fpOptN` \\ fs[fp_state_component_equality])
+    \\ first_x_assum (qspec_then `opt` assume_tac) \\ fs[]
+    \\ qexists_tac `fpOpt` \\ fs[fpState_component_equality, state_component_equality])
   (* ALL_DISTINCT (pat_bindings) *)
   >- (
-    rpt (reverse TOP_CASE_TAC \\ fs[fp_state_component_equality]))
+    rpt (reverse TOP_CASE_TAC \\ fs[fpState_component_equality, state_component_equality]))
 QED
 end
 
@@ -443,58 +443,58 @@ val prep = fn thm => SIMP_RULE std_ss [] thm;
   This is the key lemma for proving correctness of Icing optimizations
 **)
 Theorem isPureExp_evaluate_change_oracle:
-  ! (st1 st2:'a state) env fps1 fps2 e r.
+  ! (st1 st2:'a state) env e r.
     isPureExp e /\
-    evaluate st1 env fps1 [e] = (st2, fps2, Rval r) ==>
-    ! opt (stN1:'a state) fps3 g.
-      (fps3.canOpt <=> fps1.canOpt) ==>
+    evaluate st1 env [e] = (st2, Rval r) ==>
+    ! opt (stN1:'a state) g.
+      (stN1.fp_state.canOpt <=> st1.fp_state.canOpt) ==>
       ? oracle.
-        evaluate stN1 env (fps3 with <| rws := fps1.rws ++ [opt]; opts := oracle |>) [e] =
-          (stN1, fps3 with <| rws := fps1.rws ++ [opt]; opts := g; choices := fps3.choices + (fps2.choices - fps1.choices) |>, Rval r)
+        evaluate (stN1 with fp_state := stN1.fp_state with <| rws := st1.fp_state.rws ++ [opt]; opts := oracle |>) env [e] =
+          (stN1 with fp_state := stN1.fp_state with <| rws := st1.fp_state.rws ++ [opt]; opts := g; choices := stN1.fp_state.choices + (st2.fp_state.choices - st1.fp_state.choices) |>, Rval r)
 Proof
   rpt strip_tac
   (* This will come in handy later to finish the proof
      The final fs call will not conclude without this assumption being proven! *)
-  \\ `fps1.choices <= fps2.choices`
+  \\ `st1.fp_state.choices <= st2.fp_state.choices`
       by (imp_res_tac (CONJUNCT1 evaluate_fp_opts_inv)
-          \\ fs[fp_state_component_equality])
+          \\ fs[fpState_component_equality])
   (* Append the optimization *)
   \\ first_x_assum (mp_then Any assume_tac (prep (CONJUNCT1 evaluate_fp_rws_append)))
   \\ first_x_assum (qspec_then `opt` assume_tac) \\ fs[]
   (* Change the global state *)
   \\ first_x_assum (mp_then Any assume_tac (prep (CONJUNCT1 isPureExpList_swap_ffi)))
   \\ fs[isPureExp_def]
-  \\ first_x_assum (qspecl_then [`stN1`, `fps3 with <| rws := fps1.rws ++ [opt]; opts := fpOptN |>`] impl_subgoal_tac)
+  \\ first_x_assum (qspecl_then [`stN1 with fp_state := stN1.fp_state with <| rws := st1.fp_state.rws ++ [opt]; opts := fpOpt |>`] impl_subgoal_tac)
   \\ fs[]
   (* Change the resulting opts function to an arbitrary one *)
   \\ first_x_assum (mp_then Any assume_tac optUntil_evaluate_ok)
-  \\ fs[fp_state_component_equality]
-  \\ qexists_tac `optUntil (fps2.choices - fps1.choices) fpOptN g`
+  \\ fs[fpState_component_equality]
+  \\ qexists_tac `optUntil (st2.fp_state.choices - st1.fp_state.choices) fpOpt g`
   \\ first_x_assum (qspec_then `g` assume_tac)
   \\ imp_res_tac (CONJUNCT1 evaluate_fp_opts_inv)
-  \\ fs[fp_state_component_equality]
+  \\ fs[fpState_component_equality]
 QED
 
 Theorem fp_add_comm_cases:
-  ! e.
+  ! e fpBop.
     (? e1 e2.
-      e = (App (FP_bop FP_Add) [e1; e2]) /\
+      e = (App (FP_bop fpBop) [e1; e2]) /\
       isPureExp e /\
-      rewriteFPexp [fp_add_comm] (App (FP_bop FP_Add) [e1; e2]) =
-        App (FP_bop FP_Add) [e2; e1]) \/
-    (rewriteFPexp [fp_add_comm] e = e)
+      rewriteFPexp [fp_comm_gen fpBop] (App (FP_bop fpBop) [e1; e2]) =
+        App (FP_bop fpBop) [e2; e1]) \/
+    (rewriteFPexp [fp_comm_gen fpBop] e = e)
 Proof
-  rpt gen_tac \\ fs[rewriteFPexp_def, fp_add_comm_def, matchesFPexp_def]
-  \\ Cases_on `e` \\ fs[]
+  rpt gen_tac \\ Cases_on `e`
+  \\ fs[fp_comm_gen_def, rewriteFPexp_def, isPureExp_def, matchesFPexp_def]
   \\ rename1 `App op els`
-  \\ Cases_on `op` \\ fs[]
-  \\ Cases_on `f` \\ fs[] \\ EVAL_TAC
+  \\ Cases_on `op` \\ fs[isPureOp_def]
+  \\ Cases_on `fpBop` \\ fs[] \\ EVAL_TAC
 QED
 
 Theorem fp_state_opts_eq[local]:
   fps with <| rws := rwsN; opts := fps.opts |> = fps with <| rws := rwsN |>
 Proof
-  Cases_on `fps` \\ fs[fp_state_component_equality]
+  Cases_on `fps` \\ fs[fpState_component_equality]
 QED
 
 Theorem do_app_fp_inv:
@@ -518,7 +518,7 @@ local
     SIMP_RULE std_ss [] evaluate_fp_rws_append
     |> CONJ_LIST 2
     |> map (SPEC_ALL) |> map (GEN ``(opt:fp_pat #fp_pat)``)
-    |> map (Q.SPEC `fp_add_comm`) |> map GEN_ALL
+    |> map (Q.SPEC `fp_comm_gen fpBop`) |> map GEN_ALL
     |> LIST_CONJ;
   val eval_fp_opt_inv =
     SIMP_RULE std_ss [] fpSemPropsTheory.evaluate_fp_opts_inv
@@ -528,103 +528,123 @@ local
     |> CONJ_LIST 2
     |> hd
 in
-Theorem fp_add_comm_correct:
-  ! (ffi1 ffi2:'a state) env (fps1 fps2:fp_state) e res.
-    fps1.canOpt /\
-    evaluate ffi1 env fps1 [rewriteFPexp [fp_add_comm] e] = (ffi2, fps2, Rval res) ==>
+Theorem fp_comm_gen_correct:
+  ! fpBop (st1 st2:'a state) env e res.
+    st1.fp_state.canOpt /\
+    evaluate st1 env [rewriteFPexp [fp_comm_gen fpBop] e] = (st2, Rval res) ==>
     ! g. ? (fp_opts:num -> rewrite_app list).
-      evaluate ffi1 env
-        (fps1 with <| rws := fps1.rws ++ [fp_add_comm]; opts := fp_opts |>) [e] =
-        (ffi2, fps2 with <| rws := fps2.rws ++ [fp_add_comm]; opts := g |>, Rval res)
+      evaluate (st1 with fp_state := st1.fp_state with
+                <| rws := st1.fp_state.rws ++ [fp_comm_gen fpBop];
+                   opts := fp_opts |>)
+               env [e] =
+        (st2 with fp_state := st2.fp_state with
+          <| rws := st2.fp_state.rws ++ [fp_comm_gen fpBop]; opts := g |>,
+        Rval res)
 Proof
   rpt strip_tac
-  \\ qspec_then `e` assume_tac (ONCE_REWRITE_RULE [DISJ_COMM] fp_add_comm_cases)
+  \\ qspecl_then [`e`, `fpBop`] assume_tac (ONCE_REWRITE_RULE [DISJ_COMM] fp_add_comm_cases)
   \\ fs[]
   >- (
     pop_assum (fn thm => fs[thm])
     \\ imp_res_tac fp_rws_append_comm
+    \\ first_x_assum (qspec_then `fpBop` assume_tac) \\ fs[]
     \\ first_x_assum (mp_then Any (qspec_then `g` assume_tac) optUntil_evaluate_ok)
-    \\ fs[fp_state_component_equality]
+    \\ fs[fpState_component_equality]
     \\ asm_exists_tac \\ fs[])
   \\ fs[evaluate_def] \\ rveq
-  \\ qpat_x_assum `_ = (_, _, _)` mp_tac
-  \\ rename [`evaluate ffi1 env fps1 [e1]`]
-  \\ Cases_on `evaluate ffi1 env fps1 [e1]` \\ fs[]
-  \\ rename [`evaluate ffi1 env fps1 [e1] = (ffi2, r)`]
-  \\ PairCases_on `r` \\ fs[]
-  \\ rename [`evaluate ffi1 env fps1 [e1] = (ffi2, fps2, r)`]
+  \\ qpat_x_assum `_ = (_, _)` mp_tac
+  \\ rename [`evaluate st1 env [e1]`]
+  \\ Cases_on `evaluate st1 env [e1]` \\ fs[]
+  \\ rename [`evaluate st1 env [e1] = (st2, r)`]
   \\ Cases_on `r` \\ fs[]
-  \\ rename [`evaluate ffi2 env fps2 [e2]`]
-  \\ Cases_on `evaluate ffi2 env fps2 [e2]` \\ fs[]
-  \\ rename [`evaluate ffi2 env fps2 [e2] = (ffi3, r)`] \\ PairCases_on `r` \\ fs[]
-  \\ rename [`evaluate ffi2 env fps2 [e2] = (ffi3, fps3, r)`]
-  \\ Cases_on `r` \\ fs[]
+  \\ rename [`evaluate st1 env [e1] = (st2, Rval r)`]
+  \\ rename [`evaluate st2 env [e2]`]
+  \\ Cases_on `evaluate st2 env [e2]` \\ fs[]
+  \\ rename [`evaluate st2 env [e2] = (st3, r)`] \\ Cases_on `r` \\ fs[]
+  \\ rename [`evaluate st2 env [e2] = (st3, Rval r)`]
   \\ fs[astTheory.isFpOp_def, astTheory.isFpBool_def]
   \\ ntac 3 (TOP_CASE_TAC \\ fs[])
-  \\ `ffi1 = ffi2 /\ ffi2 = ffi3`
-    by (imp_res_tac isPureExp_same_ffi \\ fs[isPureExp_def])
-  \\ rveq
-  \\ `fps3.canOpt` by (imp_res_tac evaluate_fp_opts_inv \\ fs[])
+  \\ `st2 = st1 with fp_state := st2.fp_state /\ st3 = st1 with fp_state := st3.fp_state`
+    by (imp_res_tac isPureExp_same_ffi \\ fs[isPureExp_def] \\ res_tac \\ fs[state_component_equality])
+  \\ imp_res_tac evaluate_sing \\ rveq \\ fs[]
+  \\ rename [`evaluate st1 env [e1] = (st2, Rval [r1])`, `evaluate st2 env [e2] = (st3, Rval [r2])`]
+  \\ Cases_on `do_app (st3.refs, st3.ffi) (FP_bop fpBop) [r2; r1]` \\ fs[]
+  \\ PairCases_on `x` \\ fs[]
+  \\ imp_res_tac do_app_fp_inv \\ rveq \\ fs[]
+  \\ `st3.fp_state.canOpt` by (imp_res_tac evaluate_fp_opts_inv \\ fs[])
   \\ fs[]
   \\ rpt strip_tac \\ rveq
   \\ ntac 2 (first_x_assum (fn thm => (mp_then Any assume_tac isPureExp_evaluate_change_oracle thm) \\ mp_tac thm))
   \\ rpt (disch_then assume_tac)
   \\ first_x_assum
       (qspecl_then
-        [`fp_add_comm`,
-         `ffi1`,
-         `fps2 with choices := fps1.choices + (fps3.choices - fps2.choices)`,
+        [`fp_comm_gen fpBop`,
+         `st1 with fp_state := st2.fp_state with choices := st1.fp_state.choices + (st3.fp_state.choices - st2.fp_state.choices)`,
          `\x. if (x = 0)
-              then [RewriteApp Here (LENGTH fps1.rws + 1)] ++
-                    (case do_fprw r (fps3.opts x) fps3.rws of | NONE => [] | SOME r_opt => fps3.opts x) else g (x - 1)`]
-        impl_subgoal_tac)
+              then [RewriteApp Here (LENGTH st1.fp_state.rws + 1)] ++
+                (case do_fprw (Rval (FP_WordTree (fp_bop fpBop w1 w2))) (st3.fp_state.opts x) st3.fp_state.rws of | NONE => [] | SOME r_opt => st3.fp_state.opts x)
+              else g (x - 1)`]
+      impl_subgoal_tac)
   >- (fs[isPureExp_def]
       \\ imp_res_tac evaluate_fp_opts_inv \\ fs[])
   \\ fs[]
-  \\ first_x_assum (qspecl_then [`fp_add_comm`, `ffi1`, `fps1`, `oracle`] impl_subgoal_tac)
+  \\ first_x_assum (qspecl_then [`fp_comm_gen fpBop`, `st1`, `oracle`] impl_subgoal_tac)
   >- (fs[isPureExp_def]
       \\ imp_res_tac evaluate_fp_opts_inv \\ fs[])
   \\ fs[]
-  \\ `fps1.rws = fps2.rws` by (imp_res_tac evaluate_fp_opts_inv \\ fs[])
+  \\ `st1.fp_state.rws = st2.fp_state.rws` by (imp_res_tac evaluate_fp_opts_inv \\ fs[])
   \\ qexists_tac `oracle'` \\ fs[]
-  \\ `fps2 with <| rws := fps2.rws ++ [fp_add_comm]; opts := oracle; choices := fps1.choices + (fps3.choices - fps2.choices)|> =
-      fps1 with <| rws := fps1.rws ++ [fp_add_comm]; opts := oracle; choices := fps1.choices + (fps3.choices - fps2.choices)|>`
-    by (fs[fp_state_component_equality]
-        \\ imp_res_tac evaluate_fp_opts_inv \\ fs[])
+  \\ `st1 with fp_state  := st2.fp_state with
+        <| rws := st2.fp_state.rws ++ [fp_comm_gen fpBop];
+           opts := oracle;
+           choices := st1.fp_state.choices + (st3.fp_state.choices - st2.fp_state.choices) |> =
+      st1 with fp_state := st1.fp_state with
+        <| rws := st2.fp_state.rws ++ [fp_comm_gen fpBop];
+           opts := oracle;
+           choices := st1.fp_state.choices + (st3.fp_state.choices - st2.fp_state.choices) |>`
+    by (fs[fpState_component_equality, state_component_equality]
+        \\ imp_res_tac evaluate_fp_opts_inv \\ fs[]
+        \\ simp[FUN_EQ_THM])
   \\ pop_assum (fn thm => fs[thm])
-  \\ `fps2.canOpt` by (imp_res_tac evaluate_fp_opts_inv \\ fs[])
+  \\ `st2.fp_state.canOpt` by (imp_res_tac evaluate_fp_opts_inv \\ fs[])
   \\ fs[]
   \\ imp_res_tac isPureOp_same_ffi \\ fs[isPureOp_def]
-  \\ first_x_assum (qspecl_then [`ffi1.refs`, `ffi1.ffi`] assume_tac)
+  \\ first_x_assum (qspecl_then [`st1.refs`, `st1.ffi`] assume_tac)
   \\ fs[list_result_def]
-  \\ imp_res_tac evaluate_sing \\ rveq \\ fs[]
-  \\ imp_res_tac do_app_fp_inv \\ rveq
-  \\ fs[do_app_def, shift_fp_opts_def, fp_state_component_equality]
+  \\ fs[do_app_def, shift_fp_opts_def, fpState_component_equality]
   \\ rpt conj_tac
-  >- (imp_res_tac evaluate_fp_opts_inv \\ fs[])
-  >- (fs[FUN_EQ_THM])
-  >- (imp_res_tac evaluate_fp_opts_inv \\ fs[])
+  >- (imp_res_tac evaluate_fp_opts_inv \\ fs[fpState_component_equality, state_component_equality]
+      \\ conj_tac \\ simp[FUN_EQ_THM])
   \\ fs[do_fprw_def, rwAllWordTree_def, nth_len]
-  \\ fs[EVAL ``rwFp_pathWordTree fp_add_comm Here (fp_bop FP_Add w2 w1)``, instWordTree_def, substLookup_def]
-  \\ Cases_on `rwAllWordTree (fps3.opts 0) fps3.rws (fp_bop FP_Add w1 w2)` \\ fs[rwAllWordTree_def, fpValTreeTheory.fp_bop_def]
+  \\ fs[EVAL ``rwFp_pathWordTree (fp_comm_gen fpBop) Here (fp_bop fpBop w2 w1)``, instWordTree_def, substLookup_def]
+  \\ Cases_on `rwAllWordTree (st3.fp_state.opts 0) st3.fp_state.rws (fp_bop fpBop w1 w2)` \\ fs[rwAllWordTree_def, fpValTreeTheory.fp_bop_def]
   \\ imp_res_tac rwAllWordTree_append_opt
-  \\ first_x_assum (qspec_then `[fp_add_comm]` assume_tac)
-  \\ `fps3.rws = fps2.rws` by (imp_res_tac evaluate_fp_opts_inv \\ fs[])
+  \\ first_x_assum (qspec_then `[fp_comm_gen fpBop]` assume_tac)
+  \\ `st3.fp_state.rws = st2.fp_state.rws` by (imp_res_tac evaluate_fp_opts_inv \\ fs[])
   \\ fs[]
 QED
 end
 
+local
+  open semanticsTheory semanticsPropsTheory;
+in
 Theorem compile_correct:
-
-  compile (c:'a config) prog = SOME (bytes,bitmaps,c') ⇒
-   let (s,env) = THE (prim_sem_env (ffi:'ffi ffi_state)) in
-   ¬semantics_prog s env prog Fail ∧
+  compile c prog = progN ==>
+  let (s,env) = THE (prim_sem_env (ffi:'ffi ffi_state)) in
+  ¬semantics_prog s env prog Fail ==>
+  (* TODO: Side conditions???
    backend_config_ok c ∧ lab_to_targetProof$mc_conf_ok mc ∧ mc_init_ok c mc ∧
-   installed bytes cbspace bitmaps data_sp c'.lab_conf.ffi_names ffi (heap_regs c.stack_conf.reg_names) mc ms ⇒
-     (semantics_prog s env prog) ⊆
-       (* TODO: Oracle here *) (semantics_prog s env prog)
-
+   installed bytes cbspace bitmaps data_sp c'.lab_conf.ffi_names ffi (heap_regs c.stack_conf.reg_names) mc ms ⇒ *)
+    ? fpOpt.
+      (semantics_prog s env progN) ⊆
+      (semantics_prog (s with fp_state := s.fp_state with <| rws := (c.rws); opts := fpOpt |>) env prog)
 Proof
+  rw[compile_def, no_optimizations_def, optimize_def, primSemEnvTheory.prim_sem_env_eq]
+  \\ once_rewrite_tac [pred_setTheory.SUBSET_DEF]
+
+  \\ rpt strip_tac
+  \\ EVAL_TAC
+QED
 
 
 val _ = export_theory ();
